@prefix t: <https://intertextuality.org/extensions/text#> .
@prefix a: <https://intertextuality.org/extensions/artifacts#> .
@prefix : <https://intertextuality.org/abstract#> .
@prefix rdfs: <http://www.w3.org/2000/01/rdf-schema#> .
@prefix owl: <http://www.w3.org/2002/07/owl#> .

<https://intertextuality.org/extensions/text>
    a owl:Ontology ;
    owl:imports <https://intertextuality.org/extensions/artifacts> ;
    rdfs:label "Text Ontology"@en ;
    rdfs:comment "This ontology defines categories for analytic access to text on different levels: works, segments, and genres."@en .

t:Text
    a owl:Class ;
    # rdfs:subClassOf a:Artifact ;
    rdfs:label "Text"@en ;
    rdfs:comment "The class of artifacts denominated as text."@en .

t:TextSegment
    owl:intersectionOf (t:Text a:Segment) ;
    rdfs:label "Text Segment"@en ;
    rdfs:comment "A segment of a text, i.e. a passage of a single text or work."@en .

t:SingleText
    owl:intersectionOf (t:Text  a:Work) ;
    rdfs:label "Single text"@en ;
    rdfs:comment "A single text is a somehow delimited text as a whole, the kind of thing denominated with terms like book, document, work, even if it's handed down only as a fragment."@en .

t:TextGenre
    owl:intersectionOf (t:Text a:System) ;
    rdfs:label "Textual Genre"@en .

t:here
    rdfs:subPropertyOf :here ;
    rdfs:domain :IntertextualRelation ;
    rdfs:range t:Text .

t:there
    rdfs:subPropertyOf :here ;
    rdfs:domain :IntertextualRelation ;
    rdfs:range t:Text .
